x86/RelocBingenproof.v
@@ -7,7 +7,7 @@ Require Import Coqlib Maps AST lib.Integers Values.
 Require Import Events lib.Floats Memory Smallstep.
 Require Import Asm RelocProg RelocProgramBytes Globalenvs.
 Require Import Stacklayout Conventions.
-Require Import Linking Errors.
+Require Import Linking RelocProgLinking Errors.
 Require Import EncDecRet RelocBingen RelocBinDecode.
 Require Import RelocProgSemantics RelocProgSemantics1.
 Require Import TranslateInstr RelocProgSemantics2.
@@ -2091,3 +2091,6 @@ Qed.
 End PRESERVATION.
 
 End WITH_INSTR_SIZE.
+
+Instance relocbingen_transflink (instr_size: instruction -> Z): TransfLink (match_prog instr_size).
+Admitted.
