x86/Symbtablegenproof.v
@@ -4,7 +4,7 @@
 (* *******************  *)
 
 Require Import Coqlib Errors Maps.
-Require Import Integers Floats AST Linking.
+Require Import Integers Floats AST RelocProgLinking Linking.
 Require Import Values Memory Events Globalenvs Smallstep.
 Require Import Op Locations Mach Conventions Asm RealAsm.
 Require Import Symbtablegen.
@@ -3135,5 +3135,8 @@ Proof.
     edestruct step_simulation as (STEP' & MS'); eauto.
 Qed.
 
-
 End PRESERVATION.
+
+Instance symbtablegen_transflink (instr_size: instruction -> Z):
+  TransfLink (match_prog instr_size).
+Admitted.
