x86/AsmLongIntproof.v
@@ -42,3 +42,7 @@ Admitted.
 End PRESERVATION.
 
 End WITH_INSTR_SIZE.
+
+
+Instance longint_transflink: TransfLink match_prog.
+Admitted.
